{
 "cells": [
  {
   "cell_type": "markdown",
   "id": "f7be2a66",
   "metadata": {},
   "source": [
    "# Problem 2\n",
    "\n",
    "Each new term in the Fibonacci sequence is generated by adding the previous two terms. By starting with $1$ and $2$, the first $10$ terms will be:\n",
    "$$\n",
    "1, 2, 3, 5, 8, 13, 21, 34, 55, 89, \\dots\n",
    "$$\n",
    "By considering the terms in the Fibonacci sequence whose values do not exceed four million, find the sum of the even-valued terms.\n"
   ]
  },
  {
   "cell_type": "markdown",
   "id": "5e366633",
   "metadata": {},
   "source": [
    "---"
   ]
  },
  {
   "cell_type": "markdown",
   "id": "000e9fcb",
   "metadata": {},
   "source": [
    "## Solution 1: Elegant Recursion\n",
    "\n",
    "### Thought process:\n",
    "\n",
    "$\\textbf{Claim}$\n",
    "<br><br>\n",
    "Let $(F_n)_{n\\ge 0}$ be the Fibonacci sequence with $F_0=0$, $F_1=1$, and $F_{n}=F_{n-1}+F_{n-2}$.\n",
    "Then $F_{3n}$ is even and $F_{3n-1},F_{3n-2}$ are odd for all $n\\ge 1$.\n",
    "Moreover, the even subsequence $E_n := F_{3n}$ satisfies\n",
    "$$\n",
    "E_n = 4E_{n-1} + E_{n-2} \\quad (n\\ge 2),\n",
    "$$\n",
    "with $E_0=0$, $E_1=2$.\n",
    "<br><br><br>\n",
    "\n",
    "$\\textbf{Proof 1: parity pattern}$\n",
    "<br><br>\n",
    "Working in modulo $2$ $(\\mathbb{F}_2)$. The Fibonacci recurrence becomes $F_{n+2}\\equiv F_{n+1}+F_n \\pmod 2$. <br>\n",
    "Hence, by starting at $0,1$ $(WLOG)$ we obtain the repeating pattern:\n",
    "$$\n",
    "0,1,1,0,1,1,0,1,1,\\dots\n",
    "$$\n",
    "of period $3$. \n",
    "\n",
    "$\\therefore \\forall n \\in \\mathbb{N}$, $F_{3n}\\equiv 0 \\pmod 2$ are always even, and $F_{3n - 1}\\equiv 1$, $F_{3n - 2}\\equiv 1  \\pmod 2$ are always odd.\n",
    "<br><br><br>\n",
    "\n",
    "$\\textbf{Proof 2: recurrence for even terms}$\n",
    "<br><br>\n",
    "First note the identity\n",
    "$$\n",
    "F_{n+6} = 4F_{n+3} + F_n \\qquad (\\ast)\n",
    "$$\n",
    "$\\textbf{Proof:}$\n",
    "\n",
    "Recursive definition: \n",
    "$F_{n + 2} = F_{n+1} + F_{n}$\n",
    "\n",
    "Now :\n",
    "$F_{n + 6} = F_{n + 5} + F_{n + 4}$ \n",
    "\n",
    "$F_{n + 6} = F_{n + 4} + F_{n + 3} + F_{n + 4}\\\\$\n",
    "$F_{n + 6} = F_{n + 3} + F_{n + 2} + F_{n + 3} + F_{n + 3} + F_{n + 2}\\\\$\n",
    "$F_{n + 6} = 3 F_{n + 3} + F_{n + 2} + F_{n + 2}\\\\$\n",
    "$F_{n + 6} = 3 F_{n + 3} + F_{n + 2} + F_{n + 1} + F_{n}\\\\$ \n",
    "\n",
    "$F_{n + 6} = 4 F_{n + 3} + F_{n}\\qquad (\\ast)$\n",
    "\n",
    "<br>\n",
    "\n",
    "$\\therefore$ set $E_n := F_{3n}$. \n",
    "\n",
    "\n",
    "Plugging $n\\mapsto 3n-6$ into $(\\ast)$ gives\n",
    "$$\n",
    "F_{3n} = 4F_{3n-3} + F_{3n-6} \\;\\Rightarrow\\; E_n = 4E_{n-1} + E_{n-2},\\quad (n \\in \\mathbb{N})_{\\ge 2}\n",
    "$$\n",
    "with $E_0=0$ and $E_1=2$.\n",
    "<br><br><br>\n",
    "\n",
    "$\\textbf{Summation}$\n",
    "<br><br>\n",
    "Let $S_n = \\sum_{k=1}^n E_k$. \n",
    "\n",
    "Then $S_n = S_{n-1} + E_n$ with $S_0=0$,\n",
    "\n",
    "We derived a recursive formula that can be implemented straight into Python."
   ]
  }
 ],
 "metadata": {
  "kernelspec": {
   "display_name": ".venv",
   "language": "python",
   "name": "python3"
  },
  "language_info": {
   "codemirror_mode": {
    "name": "ipython",
    "version": 3
   },
   "file_extension": ".py",
   "mimetype": "text/x-python",
   "name": "python",
   "nbconvert_exporter": "python",
   "pygments_lexer": "ipython3",
   "version": "3.9.6"
  }
 },
 "nbformat": 4,
 "nbformat_minor": 5
}
